Environment.v
@@ -1,377 +1,187 @@
-Require Import Velus.Common.
+Require Import Coq.FSets.FMapPositive.
+Require Import Coq.FSets.FMapFacts.
+Require Import Coq.ZArith.ZArith.
 
-Require Import List.
-Require Import Coq.Structures.OrderedType.
-Require Import Coq.Structures.OrderedTypeEx.
+Module Env.
 
-Module POTB := PositiveOrderedTypeBits.
+  Include PositiveMap.
+  Include PositiveMapAdditionalFacts.
+  Module Props := FMapFacts.OrdProperties PositiveMap.
 
-Import List.ListNotations.
+  Section Extra.
 
-Set Implicit Arguments.
+    Context {A: Type}.
 
-Definition t (A: Type) := list (ident * A).
+    Definition adds (xs: list positive) (vs : list A) (m : t A) :=
+      fold_right (fun (xv: positive * A) env =>
+                    let (x , v) := xv in
+                    add x v env) m (combine xs vs).
 
-Section Global.
+    Lemma add_comm:
+      forall x y a b (m: t A),
+        x <> y ->
+        add x a (add y b m) = add y b (add x a m).
+    Proof.
+      induction x, y, m; simpl; intro Neq;
+        ((f_equal; apply IHx; intro Eq; apply Neq; now inversion Eq) || now contradict Neq).
+    Qed.
 
-  Variable A B: Type.
+    Lemma in_dec:
+      forall x (m: t A),
+        In x m \/ ~In x m.
+    Proof.
+      intros; destruct (Props.P.F.In_dec m x); auto.
+    Qed.
 
-  Definition empty : t A := [].
+    Remark option_map_map:
+      forall {A B C} (f: A -> B) (g: B -> C) o,
+        option_map g (option_map f o) = option_map (fun x => g (f x)) o.
+    Proof. now destruct o. Qed.
 
-  Fixpoint find (x: ident) (e: t A) : option A :=
-    match e with
-    | [] => None
-    | (y, a) :: e' =>
-      match POTB.compare x y with
-      | LT _ => None
-      | EQ _ => Some a
-      | GT _ => find x e'
-      end
-    end.
+    Lemma xmapi_xmapi:
+      forall {B C} (f: A -> B) (g: B -> C) (m: t A) x,
+        xmapi (fun _ => g) (xmapi (fun _ => f) m x) x =
+        xmapi (fun _ (x : A) => g (f x)) m x.
+    Proof.
+      induction m; intro; simpl; auto.
+      f_equal; auto.
+      apply option_map_map.
+    Qed.
 
-  Definition mem (x: ident) (e: t A) : bool :=
-    match find x e with
-    | Some _ => true
-    | None => false
-    end.
+    Lemma map_map:
+      forall {B C} (f: A -> B) (g: B -> C) (m: t A),
+        map g (map f m) = map (fun x => g (f x)) m.
+    Proof.
+      unfold map, mapi; intros.
+      apply xmapi_xmapi.
+    Qed.
 
-  Fixpoint add (x: ident) (a: A) (e: t A) : t A :=
-    match e with
-    | [] => [(x, a)]
-    | (y, b) :: e' =>
-      match POTB.compare x y with
-      | LT _ => (x, a) :: e
-      | EQ _ => (x, a) :: e'
-      | GT _ => (y, b) :: add x a e'
-      end
-    end.
+    Lemma find_gsso:
+      forall x y xs (vs: list A) m,
+        x <> y ->
+        find x (adds (y :: xs) vs m) = find x (adds xs (tl vs) m).
+    Proof.
+      intros ** Hneq.
+      unfold adds.
+      destruct vs.
+      - destruct xs; reflexivity.
+      - simpl; rewrite gso; auto.
+    Qed.
 
-  Definition map (f: A -> B) (e: t A) : t B :=
-    List.map (fun (xa: ident * A) =>
-                let (x, a) := xa in
-                (x, f a))
-             e.
+    Lemma find_gsss:
+      forall x a xs (vs: list A) m,
+        find x (adds (x :: xs) (a :: vs) m) = Some a.
+    Proof.
+      intros; unfold adds; apply gss.
+    Qed.
 
-  Definition mapi (f: ident -> A -> B) (e: t A) : t B :=
-    List.map (fun (xa: ident * A) =>
-                let (x, a) := xa in
-                (x, f x a))
-             e.
+    Lemma find_In_gsso:
+      forall x xs (vs: list A) m,
+        ~ List.In x xs ->
+        find x (adds xs vs m) = find x m.
+    Proof.
+      intros ** Hin.
+      revert vs; induction xs; intro; simpl; auto.
+      rewrite find_gsso.
+      - apply IHxs; intuition.
+      - intro; apply Hin; now left.
+    Qed.
 
-  (* Function eqb (cmp: A -> A -> bool) (e e' : t A) {struct e} : bool := *)
-  (*   match e, e' with *)
-  (*   | [], [] => true *)
-  (*   | (x, a) :: e, (x', a') :: e' => *)
-  (*     match POTB.compare x x' with *)
-  (*      | EQ _ => cmp a a' && eq cmp e e' *)
-  (*      | _ => false *)
-  (*     end *)
-  (*  | _, _ => false *)
-  (* end. *)
+    Lemma find_gssn:
+      forall d1 (d2: A) n m xs vs x,
+        n < length xs ->
+        length xs = length vs ->
+        NoDup xs ->
+        nth n xs d1 = x ->
+        find x (adds xs vs m) = Some (nth n vs d2).
+    Proof.
+      intros ** Hlen Hleq Hndup Hnth.
+      unfold adds.
+      remember (combine xs vs) as xvs eqn:Hxvs.
+      assert (xs = fst (split xvs)) as Hxs
+          by (now subst xvs; rewrite combine_split with (1:=Hleq)).
+      assert (vs = snd (split xvs)) as Hvs
+          by (now subst xvs; rewrite combine_split with (1:=Hleq)).
+      subst xs vs.
+      clear Hleq. revert n Hlen Hnth.
+      induction xvs as [|xv xvs]; intros n Hlen Hnth.
+      now inversion Hlen.
+      simpl. destruct xv as [x' v'].
+      simpl in *; destruct (split xvs); simpl in *.
+      inversion_clear Hndup as [|? ? Hnin Hndup'].
+      destruct n.
+      - subst. now rewrite gss.
+      - injection Hxvs; intro; subst.
+        rewrite gso.
+        + rewrite (IHxvs Hndup' eq_refl n); auto with arith.
+        + pose proof (nth_In l d1 (Lt.lt_S_n _ _ Hlen)) as Hin.
+          intro Hnth. rewrite Hnth in Hin. contradiction.
+    Qed.
 
-  Definition eq (e e' : t A) : Prop := forall x, find x e = find x e'.
+    Lemma NotIn_find_adds:
+      forall x xs (o: option A) vs m,
+        ~ List.In x xs ->
+        find x m = o ->
+        find x (adds xs vs m) = o.
+    Proof.
+      induction xs as [|xty xs]; auto.
+      intros v vs S Hnin Hfind.
+      apply Decidable.not_or in Hnin as [Hnin Hneq].
+      rewrite find_gsso; auto.
+    Qed.
 
-  Lemma eq_refl: reflexive _ eq.
-  Proof.
-    intros ?; unfold eq; reflexivity.
-  Qed.
+    Lemma adds_cons_cons:
+      forall xs x (a: A) vs m,
+        ~ List.In x xs ->
+        adds (x :: xs) (a :: vs) m = adds xs vs (add x a m).
+    Proof.
+      unfold adds.
+      induction xs as [|x']; intros ** NotIn; simpl; auto.
+      destruct vs as [|v']; simpl; auto.
+      rewrite <-IHxs.
+      - simpl.
+        rewrite add_comm; auto.
+        intro Eq.
+        apply NotIn; subst.
+        apply in_eq.
+      - apply Decidable.not_or in NotIn as []; auto.
+    Qed.
 
-  Lemma eq_symm: symmetric _ eq.
-  Proof.
-    intros ? ?; unfold eq; auto.
-  Qed.
+    Lemma adds_comm:
+      forall xs x y (a b: A) vs m,
+        ~ List.In x xs ->
+        ~ List.In y xs ->
+        x <> y ->
+        adds (x :: y :: xs) (a :: b :: vs) m = adds (y :: x :: xs) (b :: a :: vs) m.
+    Proof.
+      intros.
+      repeat rewrite adds_cons_cons; auto.
+      - rewrite add_comm; auto.
+      - intros []; contradiction.
+      - intros [|]; congruence.
+    Qed.
 
-  Lemma eq_trans: transitive _ eq.
-  Proof.
-    intros ? ? ?; unfold eq; intros E1 E2 e.
-    now rewrite E1, E2.
-  Qed.
+    Lemma adds_nil_nil:
+      forall e,
+        adds List.nil List.nil e = e.
+    Proof. unfold adds; simpl; auto. Qed.
 
-  Add Parametric Relation : (t A)  eq
-      reflexivity proved by eq_refl
-      symmetry proved by eq_symm
-      transitivity proved by eq_trans
-        as Eq_eq.
+    Lemma In_find:
+      forall x (s: t A),
+        In x s <-> (exists v, find x s = Some v).
+    Proof.
+      setoid_rewrite Props.P.F.in_find_iff; reflexivity.
+    Qed.
 
-  Fact compare_eq:
-    forall x,
-    exists H, POTB.compare x x = EQ H.
-  Proof.
-    intros; destruct (POTB.compare x x) as [|Eq|];
-      try (now exfalso; eapply POTB.bits_lt_antirefl; eauto).
-    exists Eq; auto.
-  Qed.
+    Lemma elements_In:
+      forall x (a: A) m,
+        List.In (x, a) (elements m) -> In x m.
+    Proof.
+      intros ** Hin.
+      apply elements_complete in Hin.
+      apply In_find; eauto.
+    Qed.
 
-  Theorem gss:
-    forall x a e,
-      find x (add x a e) = Some a.
-  Proof.
-    induction e as [|[y]]; simpl.
-    - destruct (compare_eq x) as [? E]; now rewrite E.
-    - destruct (POTB.compare x y) eqn: Cmp; simpl.
-      + destruct (compare_eq x) as [? E]; now rewrite E.
-      + destruct (compare_eq x) as [? E]; now rewrite E.
-      + now rewrite Cmp.
-  Qed.
+  End Extra.
 
-  Corollary gss':
-    forall x y a e,
-      ident_eqb x y = true ->
-      find x (add y a e) = Some a.
-  Proof.
-    intros ** E; rewrite ident_eqb_eq in E; subst; apply gss.
-  Qed.
-
-  Theorem gso:
-    forall x y a e,
-      x <> y ->
-      find x (add y a e) = find x e.
-  Proof.
-    induction e as [|[z]]; intros Neq; simpl.
-    - destruct (POTB.compare x y); simpl; auto.
-      now contradict Neq.
-    - destruct (POTB.compare y z) eqn: Eyz, (POTB.compare x z) eqn: Exz, (POTB.compare x y) eqn: Exy;
-        simpl; try rewrite Exy; try rewrite Exz; auto;
-          try (now contradict Neq);
-          try repeat match goal with
-                H: POTB.eq ?a ?b |- _ =>
-                assert (a = b); auto; subst b;
-                  exfalso; apply (POTB.bits_lt_antirefl a);
-                    etransitivity; eauto
-              end.
-      exfalso; apply (POTB.bits_lt_antirefl x);
-        do 2 (etransitivity; eauto).
-  Qed.
-
-  Corollary gso':
-    forall x y a e,
-      ident_eqb x y = false ->
-      find x (add y a e) = find x e.
-  Proof.
-    intros ** E; rewrite ident_eqb_neq in E; now apply gso.
-  Qed.
-
-  Lemma find_cons_eq:
-    forall x a e,
-      find x ((x, a) :: e) = Some a.
-  Proof.
-    intros; simpl.
-    destruct (compare_eq x) as [? E]; now rewrite E.
-  Qed.
-
-  Lemma find_cons_lt:
-    forall x y a e,
-      POTB.lt x y ->
-      find x ((y, a) :: e) = None.
-  Proof.
-    intros ** E; simpl.
-    destruct (POTB.compare x y) eqn: Exy; auto.
-    - assert (x = y); auto; subst; contradict E; apply POTB.bits_lt_antirefl.
-    - exfalso; apply (POTB.bits_lt_antirefl x);
-        do 2 (etransitivity; eauto).
-  Qed.
-
-  Theorem find_in:
-    forall x a e,
-      find x e = Some a ->
-      In (x, a) e.
-  Proof.
-    induction e as [|(y, b)]; simpl.
-    - intro; discriminate.
-    - intro H; destruct (POTB.compare x y); try discriminate.
-      + assert (x = y); auto; inv H; auto.
-      + right; auto.
-  Qed.
-
-  Definition add_list (xvs: list (ident * A)) (e: t A) :=
-    fold_right (fun (xv: ident * A) env =>
-                  let (x , v) := xv in
-                  add x v env) e xvs.
-
-  Definition adds xs (vs : list A) :=
-    add_list (combine xs vs).
-
-  Definition from_list (xvs: list (ident * A)) :=
-    add_list xvs empty.
-
-  Lemma add_comm:
-    forall x x' (v v': A) m,
-      x <> x' ->
-      add x v (add x' v' m) = add x' v' (add x v m).
-  Proof.
-    Ltac aux :=
-      try match goal with
-          (* | H: POTB.lt ?x' ?y, H': POTB.lt ?y ?x, H'': POTB.lt ?x ?x' |- _ => *)
-          (*   let E := fresh in *)
-          (*   assert (POTB.lt x' x) by (now transitivity y); *)
-          (*   assert (POTB.lt x' x') as E by (now transitivity x); *)
-          (*   apply POTB.lt_not_eq in E; exfalso; apply E; reflexivity *)
-          | H: POTB.lt ?x ?x', H': POTB.eq ?x' ?x |- _ =>
-            apply POTB.lt_not_eq in H; symmetry in H'; contradiction
-          | H: POTB.lt ?x ?x', H': POTB.eq ?x ?x' |- _ =>
-            apply POTB.lt_not_eq in H; contradiction
-          | H: POTB.lt ?x ?x', H': POTB.lt ?x' ?x |- _ =>
-            let E := fresh in
-            assert (POTB.lt x x) as E by (now transitivity x');
-            apply POTB.lt_not_eq in E; exfalso; apply E; reflexivity
-          | H: POTB.lt ?x ?x', H': POTB.lt ?x' ?y, H'': POTB.eq ?x ?y |- _ =>
-            let E := fresh in
-            assert (POTB.lt x y) as E by (now transitivity x');
-            apply POTB.lt_not_eq in E; contradiction
-          | H: POTB.lt ?x ?x', H': POTB.lt ?x' ?y, H'': POTB.eq ?y ?x |- _ =>
-            let E := fresh in
-            assert (POTB.lt x y) as E by (now transitivity x');
-            apply POTB.lt_not_eq in E; symmetry in H''; contradiction
-          | H: ?x <> ?x', H': POTB.eq ?x' ?y, H'': POTB.eq ?x ?y |- _ =>
-            exfalso; apply H; now rewrite H', H''
-          | H: ?x <> ?x', H': POTB.eq ?x' ?x |- _ =>
-            exfalso; apply H; now rewrite H'
-          | H: POTB.eq ?x' ?y, H': POTB.lt ?y ?x, H'': POTB.lt ?x ?x' |- _ =>
-            rewrite H in H'';
-            let E := fresh in
-            assert (POTB.lt x x) as E by (now transitivity y);
-            apply POTB.lt_not_eq in E; exfalso; apply E; reflexivity
-           end; try contradiction; auto.
-
-    intros ** Neq.
-    revert dependent x; revert v v' x'; induction m as [|(y, w)]; simpl; intros.
-    - destruct (POTB.compare x x'), (POTB.compare x' x); aux.
-    - destruct (POTB.compare x' y) eqn: E, (POTB.compare x y) eqn: E'; simpl;
-        try rewrite E; try rewrite E'; try (f_equal; auto);
-          try destruct (POTB.compare x x'); try destruct (POTB.compare x' x); aux.
-      + assert (POTB.lt x' x) by (now transitivity y);
-          assert (POTB.lt x' x') as E'' by (now transitivity x);
-          apply POTB.lt_not_eq in E''; exfalso; apply E''; reflexivity.
-      + assert (POTB.lt y x) by (now transitivity x');
-          assert (POTB.lt y y) as E'' by (now transitivity x);
-          apply POTB.lt_not_eq in E''; exfalso; apply E''; reflexivity.
-  Qed.
-
-  Lemma add_list_cons_cons:
-    forall x (v: A) xvs e,
-      ~ InMembers x xvs ->
-      add_list ((x, v) :: xvs) e = add_list xvs (add x v e).
-  Proof.
-    unfold add_list.
-    induction xvs as [|(x', v')]; intros ** NotIn; simpl; auto.
-    rewrite <-IHxvs.
-    - simpl.
-      rewrite add_comm; auto.
-      intro Eq.
-      apply NotIn; subst.
-      now constructor.
-    - apply NotInMembers_cons in NotIn; tauto.
-  Qed.
-
-  Lemma adds_cons_cons:
-    forall xs x (v: A) vs e,
-      ~ In x xs ->
-      adds (x :: xs) (v :: vs) e = adds xs vs (add x v e).
-  Proof.
-    unfold adds; intros ** NotIn.
-    apply add_list_cons_cons.
-    intro; eapply NotIn, InMembers_In_combine; eauto.
-  Qed.
-
-  Lemma find_gsso:
-    forall x x' xs (vs: list A) S,
-      x <> x' ->
-      find x (adds (x' :: xs) vs S) = find x (adds xs (tl vs) S).
-  Proof.
-    intros ** Hneq.
-    unfold adds.
-    destruct vs. destruct xs; reflexivity.
-    simpl. rewrite gso; auto.
-  Qed.
-
-  Lemma not_In_find_adds:
-    forall x xs (v: option A) vs S,
-      ~In x xs ->
-      find x S = v ->
-      find x (adds xs vs S) = v.
-  Proof.
-    induction xs as [|xty xs]; auto.
-    intros v vs S Hnin Hfind.
-    apply not_in_cons in Hnin.
-    destruct Hnin as [Hnin Hneq].
-    rewrite find_gsso; auto.
-  Qed.
-
-  Lemma In_find_add_list:
-    forall x v xvs S,
-      NoDupMembers xvs ->
-      In (x, v) xvs ->
-      find x (add_list xvs S) = Some v.
-  Proof.
-    induction xvs as [|(x', v') xvs]; try contradiction.
-    inversion_clear 1; inversion_clear 1 as [E|]; simpl.
-    - inv E; now rewrite gss.
-    - rewrite gso; auto.
-      eapply InMembers_neq; eauto.
-      eapply In_InMembers; eauto.
-  Qed.
-
-  Lemma In_find_add_list':
-    forall x v xvs S,
-      NoDupMembers xvs ->
-      find x S = None ->
-      find x (add_list xvs S) = Some v ->
-      In (x, v) xvs.
-  Proof.
-    induction xvs as [|(x', v') xvs]; simpl.
-    - intros ** ->; discriminate.
-    - inversion_clear 1; intros ** Find.
-      destruct (ident_eq_dec x x').
-      + subst; rewrite gss in Find; inv Find; auto.
-      + rewrite gso in Find; auto.
-        right; eauto.
-  Qed.
-
-  Add Parametric Morphism x v: (add x v)
-      with signature eq ==> eq
-        as add_eq.
-  Proof.
-    unfold eq; intros ** y.
-    destruct (ident_eq_dec x y).
-    - subst; now rewrite 2 gss.
-    - rewrite 2 gso; auto.
-  Qed.
-
-  Add Parametric Morphism xvs: (add_list xvs)
-      with signature eq ==> eq
-        as add_list_eq.
-  Proof.
-    unfold add_list.
-    induction xvs as [|(y, a)]; intros ** E x; simpl; auto.
-    erewrite add_eq.
-    Focus 2.
-    apply IHxvs; eauto.
-    auto.
-  Qed.
-
-  Lemma add_ps_from_list_cons:
-    forall xvs x v,
-      eq (add x v (from_list xvs))
-         (from_list ((x, v) :: xvs)).
-  Proof.
-    intros; unfold from_list; reflexivity.
-  Qed.
-
-End Global.
-
-Theorem find_map:
-  forall (A B: Type) (x: ident) (e: t A) (f: A -> B),
-    find x (map f e) = option_map f (find x e).
-Proof.
-  induction e as [|[y]]; simpl; intros; auto.
-  destruct (POTB.compare x y); auto.
-Qed.
-
-Theorem find_mapi:
-  forall (A B: Type) (x: ident) (e: t A) (f: ident -> A -> B),
-    find x (mapi f e) = option_map (f x) (find x e).
-Proof.
-  induction e as [|[y]]; simpl; intros; auto.
-  destruct (POTB.compare x y); auto.
-  assert (x = y); auto; subst; auto.
-Qed.
+End Env.
