RMemory.v
@@ -1,10 +1,8 @@
 Require Import Velus.Common.
 
-(* Require Import Coq.FSets.FMapPositive. *)
 Require Import List.
 Import List.ListNotations.
 
-Require Velus.Environment.
 Set Implicit Arguments.
 
 (** * Memory *)
@@ -21,239 +19,16 @@ Set Implicit Arguments.
 
 (** ** Datatype *)
 
-Module Env := Environment.
-
 Definition env := Env.t.
 
 Inductive memory (V: Type) :=
-  Mnode: env V -> env (memory V) -> memory V.
+  Mem {
+      values: env V;
+      instances: env (memory V)
+    }.
 
-Definition values (V: Type) (m: memory V) : env V :=
-  match m with Mnode xvs _ => xvs end.
-
-Definition instances (V: Type) (m: memory V) : env (memory V) :=
-  match m with Mnode _ xms => xms end.
-
-Section memory_ind'.
-  Variable V: Type.
-  Variable P: memory V -> Prop.
-
-  Hypothesis MnodeCase:
-    forall xvs xms,
-      Forall P (map snd xms) ->
-      P (Mnode xvs xms).
-
-  Fixpoint memory_ind' (m : memory V): P m.
-  Proof.
-    destruct m as [? xms].
-    apply MnodeCase.
-    induction xms; simpl; auto.
-  Qed.
-
-End memory_ind'.
-
-(* Require Coq.FSets.FMapList. *)
-(* Module PML := Coq.FSets.FMapList.Make Coq.Structures.OrderedTypeEx.PositiveOrderedTypeBits. *)
-
-(* Check PML.find. *)
-
-(* Inductive mem (A: Type): Type := *)
-(*     { *)
-(*       mems : PML.t A; *)
-(*       insts : PML.t (mem A) *)
-(*     }. *)
-
-
-
-(* Fixpoint tree_ind' (A : Type) (P : tree A -> Prop) *)
-(*          (H: forall n ts, *)
-(*              Forall P (map snd ts) -> *)
-(*              P {| node := n; children := ts |}) *)
-(*          (t : tree A) : P t. *)
-(* Proof. *)
-(*   destruct t as [n ts]. *)
-(*   apply H. *)
-(*   induction ts. *)
-(*   - simpl. apply Forall_nil. *)
-(*   - simpl. apply Forall_cons. *)
-(*     + apply tree_ind'. *)
-(*       exact H. *)
-(*     + exact IHts. *)
-(* Qed. *)
-
-(* Fixpoint size (A: Type) (t: tree A) : nat := *)
-  (* fold_left (fun s t => s + size (snd t)) (children t) 1. *)
-
-(* =memory= *)
-(* Inductive memory (V: Type): Type := mk_memory { *)
-(*   mm_values : PM.t V; *)
-(*   mm_instances : PM.t (memory V) }. *)
-(* =end= *)
-
-(* Check mk_memory. *)
-(* Require Import Coq.FSets.FMapFacts. *)
-
-(* Module Import PMProp := Properties PM. *)
-
-(* Fixpoint depth (V: Type) (m: memory V) : nat := *)
-(*   match PM.elements (m.(mm_instances)) with *)
-(*   | [] => 0 *)
-(*   | (_, m) :: _ => 1 + depth m *)
-(*   end. *)
-
-(* Require Import Program. *)
-(* Definition app_snd (A B C: Type) (f: B -> C) (x: A * B) := f (snd x). *)
-(* Definition instances (V: Type) (ms: PM.t (memory V)) := map snd (PM.elements ms).  *)
-(* Inductive memory' (V: Type): Type := *)
-(*   MNode: PM.t V -> PM.t (memory' V) -> memory' V. *)
-
-(* Check memory'_ind. *)
-
-(* Section MemoryInd. *)
-(*   Variable V: Type. *)
-(*   Variable P: memory' V -> Prop. *)
-
-(*   Hypothesis H: *)
-(*     forall (vs : PM.t V) (ms : PM.t (memory' V)), *)
-(*       (forall x m', PM.find x ms = Some m' -> P m') -> *)
-(*       P (MNode vs ms). *)
-
-(*   Print Forall_cons. *)
-(*   Print map_induction_bis. *)
-
-(*   Fixpoint memory_ind' (m: memory' V):  P m. *)
-(*   Proof. *)
-(*     induction m as [vs ms]. *)
-(*     apply H. *)
-(*     induction ms as [?? Eq| |] using map_induction_bis. *)
-(*     - unfold PM.Equal in Eq. *)
-(*       intros ** Find. *)
-(*       eapply IHms1; rewrite Eq; eauto. *)
-(*     - intros ** Find. *)
-(*       rewrite PM.gempty in Find; discriminate. *)
-(*     - intros y ** Find. *)
-(*       destruct (ident_eq_dec y x). *)
-(*       + subst. *)
-(*         rewrite PM.gss in Find. *)
-(*         apply memory_ind'. *)
-(*       + rewrite PM.gso in Find; auto. *)
-(*         Show Proof. *)
-(*   Defined. *)
-
-
-(*     := *)
-(*     match m with *)
-(*       MNode vs ms => *)
-(*       H vs ms *)
-(*         (map_induction_bis *)
-(*            (P := fun ms0 : PM.t (memory' V) => forall (x : positive) (m' : memory' V), PM.find x ms0 = Some m' -> P m') *)
-(*            (fun (ms1 ms2 : PM.t (memory' V)) (Eq : PM.Equal ms1 ms2) *)
-(*               (IHms1 : forall (x : positive) (m' : memory' V), PM.find x ms1 = Some m' -> P m')  *)
-(*               (x : positive) (m' : memory' V) (Find : PM.find x ms2 = Some m') => *)
-(*               IHms1 x m' (eq_ind_r (fun o : option (memory' V) => o = Some m') Find (Eq x))) *)
-(*            (fun (x : positive) (m' : memory' V) (Find : PM.find x (PM.empty (memory' V)) = Some m') => *)
-(*               (fun Find0 : None = Some m' => *)
-(*                  (fun H0 : False => (fun H1 : False => False_ind (P m') H1) H0) *)
-(*                    (eq_ind None (fun e : option (memory' V) => match e with *)
-(*                                                             | Some _ => False *)
-(*                                                             | None => True *)
-(*                                                             end) I  *)
-(*                            (Some m') Find0)) *)
-(*                 (eq_ind (PM.find x (PM.empty (memory' V)))  *)
-(*                         (fun o : option (memory' V) => o = Some m') Find None  *)
-(*                         (PM.gempty (memory' V) x))) *)
-(*            (fun (x : PM.key) (e : memory' V) (ms0 : PM.t (memory' V))  *)
-(*               (_ : ~ PM.In x ms0) (IHms : forall (x0 : positive) (m' : memory' V), PM.find x0 ms0 = Some m' -> P m') *)
-(*               (y : positive) (m' : memory' V) (Find : PM.find y (PM.add x e ms0) = Some m') => *)
-(*               let s := ident_eq_dec y x in *)
-(*               match s with *)
-(*               | left e0 => *)
-(*                 eq_ind_r (fun y0 : positive => PM.find y0 (PM.add x e ms0) = Some m' -> P m') *)
-(*                          (fun Find0 : PM.find x (PM.add x e ms0) = Some m' => *)
-(*                             (fun _ : Some e = Some m' => memory_ind' m') *)
-(*                               (eq_ind (PM.find x (PM.add x e ms0))  *)
-(*                                       (fun o : option (memory' V) => o = Some m') Find0  *)
-(*                                       (Some e) (PM.gss x e ms0))) e0 Find *)
-(*               | right n => *)
-(*                 (fun Find0 : PM.find y ms0 = Some m' => IHms y m' Find0) *)
-(*                   (eq_ind (PM.find y (PM.add x e ms0))  *)
-(*                           (fun o : option (memory' V) => o = Some m') Find  *)
-(*                           (PM.find y ms0) (PM.gso e ms0 n)) *)
-(*               end) ms) *)
-(*     end. *)
-
-(*     match m with *)
-(*       MNode vs ms => *)
-(*       H vs ms *)
-(*         (let l := map snd (PM.elements ms) in *)
-(*          (fix list_ind' (ms: list (memory' V)): Forall P ms := *)
-(*             match ms with *)
-(*             | [] => Forall_nil P *)
-(*             | m :: ms => *)
-(*               Forall_cons m (memory_ind' m) (list_ind' ms) *)
-(*             end) l) *)
-(*     end. *)
-
-(* Section MemoryInd. *)
-(*   Variable V: Type. *)
-(*   Variable P: memory' V -> Prop. *)
-
-(*   Hypothesis H: *)
-(*     forall (vs : PM.t V) (ms : PM.t (memory' V)), *)
-(*       Forall P (map snd (PM.elements ms)) -> *)
-(*       P (MNode vs ms). *)
-
-(*   Print Forall_cons. *)
-
-(*   Fixpoint memory_ind' (m: memory' V):  P m := *)
-(*     match m with *)
-(*       MNode vs ms => *)
-(*       H vs ms *)
-(*         (let l := map snd (PM.elements ms) in *)
-(*          (fix list_ind' (ms: list (memory' V)): Forall P ms := *)
-(*             match ms with *)
-(*             | [] => Forall_nil P *)
-(*             | m :: ms => *)
-(*               Forall_cons m (memory_ind' m) (list_ind' ms) *)
-(*             end) l) *)
-(*     end. *)
-
-(* Proof. *)
-(*   destruct m as [vs ms]. *)
-(*   apply H. *)
-(*   induction (PM.elements ms) as [|[? m]]; auto. *)
-(* Qed. *)
-
-(*   constructor; auto. *)
-(*   simpl; apply memory_ind'. apply H. *)
-(* Admitted. *)
-
-(* End MemoryInd. *)
-
-(* Fixpoint memory_ind'' (V : Type) (P : memory V -> Prop) *)
-(*          (H: forall (vs : PM.t V) (ms : PM.t (memory V)), *)
-(*              (forall x m', PM.find x ms = Some m' -> P m') -> *)
-(*              P {| mm_values := vs; mm_instances := ms |}) (m : memory V) {struct m} : P m. *)
-(* Proof. *)
-(*   destruct m as [vs ms]. *)
-(*   apply H. *)
-(*   induction ms as [?? Eq| |] using map_induction_bis. *)
-(*   - unfold PM.Equal in Eq. *)
-(*     intros ** Find. *)
-(*     eapply IHms1; rewrite Eq; eauto. *)
-(*   - intros ** Find. *)
-(*     rewrite PM.gempty in Find; discriminate. *)
-(*   - intros y ** Find. *)
-(*     destruct (ident_eq_dec y x). *)
-(*     + subst. *)
-(*       rewrite PM.gss in Find. *)
-(*       apply memory_ind''. *)
-(*       auto. *)
-(*     + rewrite PM.gso in Find; auto. *)
-(*       eapply IHms; eauto. *)
-(* Qed. *)
-
-(* Admitted. *)
+Definition max (l: list nat) : nat :=
+  fold_left (fun m x => if NPeano.leb x m then m else x) l 0.
 
 (** ** Operations *)
 
@@ -261,7 +36,7 @@ Section Operations.
 
   Variable V W: Type.
 
-  Definition empty_memory : memory V := Mnode [] [].
+  Definition empty_memory : memory V := Mem (Env.empty V) (Env.empty (memory V)).
 
   Definition find_val (x: ident) (m: memory V) : option V :=
     Env.find x (values m).
@@ -273,21 +48,51 @@ Section Operations.
     find_inst x m = Some m'.
 
   Definition add_val (x: ident) (v: V) (m: memory V) : memory V :=
-    Mnode (Env.add x v (values m)) (instances m).
+    Mem (Env.add x v (values m)) (instances m).
 
   Definition add_vals (xs: list ident) (vs: list V) (m: memory V) : memory V :=
-    Mnode (Env.adds xs vs (values m)) (instances m).
+    Mem (Env.adds xs vs (values m)) (instances m).
 
   Definition add_inst (x: ident) (m': memory V) (m: memory V) : memory V :=
-    Mnode (values m) (Env.add x m' (instances m)).
+    Mem (values m) (Env.add x m' (instances m)).
 
   Fixpoint mmap (f: V -> W) (m: memory V) : memory W :=
-    Mnode (Env.map f (values m)) (Env.map (mmap f) (instances m)).
+    Mem (Env.map f (values m)) (Env.map (mmap f) (instances m)).
 
-  Fixpoint mmapi (f: list ident -> ident -> V -> W) (p: list ident) (m: memory V) : memory W :=
-    Mnode (Env.mapi (f p) (values m)) (Env.mapi (fun i => mmapi f (p ++ [i])) (instances m)).
+  (* Fixpoint mmapi (f: list ident -> ident -> V -> W) (p: list ident) (m: memory V) : memory W := *)
+  (*   Mnode (Env.mapi (f p) (values m)) (Env.mapi (fun i => mmapi f (p ++ [i])) (instances m)). *)
 
 End Operations.
+
+(** ** Induction Scheme *)
+
+Section MemoryInd.
+
+  Variable V: Type.
+  Variable P: memory V -> Prop.
+
+  Hypothesis MemCase:
+    forall m,
+      (forall m' x, sub_inst x m m' -> P m') ->
+      P m.
+
+  Fixpoint memory_ind' (m : memory V): P m.
+  Proof.
+    unfold sub_inst, find_inst in MemCase.
+    destruct m as [? xms].
+    apply MemCase; simpl.
+    induction xms; intros ** Find.
+    - rewrite Env.gleaf in Find; discriminate.
+    - destruct x; simpl in Find.
+      + eapply IHxms2; eauto.
+      + eapply IHxms1; eauto.
+      + destruct o.
+        * symmetry in Find; inv Find. apply memory_ind'.
+        * discriminate.
+  Qed.
+
+End MemoryInd.
+
 
 (** ** Properties *)
 
@@ -348,34 +153,34 @@ Section Properties.
   Proof.
     unfold find_val.
     destruct m; simpl.
-    apply Env.find_map.
+    apply Env.Props.P.F.map_o.
   Qed.
 
-  Lemma find_val_mmapi:
-    forall (f: list ident -> ident -> V -> W) p,
-      find_val x (mmapi f p m) = option_map (f p x) (find_val x m).
-  Proof.
-    intros; unfold find_val.
-    destruct m; simpl.
-    apply Env.find_mapi.
-  Qed.
+  (* Lemma find_val_mmapi: *)
+  (*   forall (f: list ident -> ident -> V -> W) p, *)
+  (*     find_val x (mmapi f p m) = option_map (f p x) (find_val x m). *)
+  (* Proof. *)
+  (*   intros; unfold find_val. *)
+  (*   destruct m; simpl. *)
+  (*   apply Env.find_mapi. *)
+  (* Qed. *)
 
   Lemma find_inst_mmap:
     find_inst x (mmap f m) = option_map (mmap f) (find_inst x m).
   Proof.
     unfold find_inst.
     destruct m; simpl.
-    apply Env.find_map.
+    apply Env.Props.P.F.map_o.
   Qed.
 
-  Lemma find_inst_mmapi:
-    forall (f: list ident -> ident -> V -> W) p,
-      find_inst x (mmapi f p m) = option_map (mmapi f (p ++ [x])) (find_inst x m).
-  Proof.
-    intros; unfold find_inst.
-    destruct m; simpl.
-    apply Env.find_mapi.
-  Qed.
+  (* Lemma find_inst_mmapi: *)
+  (*   forall (f: list ident -> ident -> V -> W) p, *)
+  (*     find_inst x (mmapi f p m) = option_map (mmapi f (p ++ [x])) (find_inst x m). *)
+  (* Proof. *)
+  (*   intros; unfold find_inst. *)
+  (*   destruct m; simpl. *)
+  (*   apply Env.find_mapi. *)
+  (* Qed. *)
   (* Lemma values_mmap: *)
   (*   Env.map f (values m) = values (mmap f m). *)
   (* Proof. *)
